decomented parts of PureITreeSpec, developed specification monad for state itrees

theories/Dijkstra/ItreeDijkstra.v
@@ -32,6 +32,7 @@ Import MonadNotation.
 Local Open Scope monad_scope.
 Local Open Scope string_scope.
 
+(** The itree Tau (Tau (Tau ...))*)
 CoFixpoint spin {E: Type -> Type} {A : Type}  : itree E A := Tau spin.
 
 Lemma spin_div : forall E A, @divergence E A spin.
@@ -48,35 +49,14 @@ Proof.
 Qed.
 
 Inductive Void : Type -> Type := .
+
+(*Depreacated predicate on itree predicates. Intended to denote that a predicate is invariant wrt adding
+  or subtracting a finite number of Tau's. Replaced with resp_eutt*)
 Definition tau_invar (E : Type -> Type) (A : Type) (P : itree E A -> Prop) : Prop :=
     forall (t : itree E A), (P t -> (P (Tau t))) /\(P (Tau t) -> P t).
-(* maybe  *)
-Inductive resp_euttF  {E : Type -> Type} {A : Type} (F : (itree E A -> Prop) -> Prop)  (P : itree E A -> Prop): Prop :=
-  resp_eutt_intro (t1 t2 : itree E A) (Heutt : t1 ≈ t2) (Hiff : P t1 <-> P t2).
 
-Hint Constructors resp_euttF.
-                  
-Definition resp_eutt_ {E A} sim :=
-  fun P => @resp_euttF E A sim P.
-
-Hint Unfold resp_eutt_.
-
-Lemma resp_euttF_mono {E A} sim sim' P (IN : resp_euttF sim P) (LE : sim <1= sim') :
-  @resp_euttF E A sim' P.
-Proof.
-  induction IN; eauto.
-Qed.
-
-Lemma resp_euttF_mono' {E A} : monotone1 (@resp_euttF E A).
-Proof.
-  unfold monotone1. intros.
-  eapply resp_euttF_mono; eauto.
-Qed.
-
-Hint Resolve resp_euttF_mono' : paco.
-
-Definition resp_eutt' {E A} := paco1 (@resp_euttF E A) bot1.
-
+(*Characterizes predicates that respect the eutt relation on itrees. Captures the notion that a predicate
+  is invariant wrt adding or subtracting a finite number of Tau's*)
 Definition resp_eutt (E : Type -> Type) (A : Type) (P : itree E A -> Prop) : Prop :=
   forall (t1 t2 : itree E A), t1 ≈ t2 -> (P t1 <-> P t2).
 
@@ -86,33 +66,25 @@ Lemma tau_invar_resp_eutt1: forall (E : Type -> Type) (A : Type) (P : itree E A 
     intros. unfold tau_invar. split; intros;
     eapply H; try eassumption; rewrite tau_eutt; reflexivity.
   Qed.
-(* not sure that did anything
-Lemma tau_invar_resp_eutt2_aux : forall (A : Type) (P : itree Void A -> Prop),
-      tau_invar Void A P -> resp_eutt' P.
-  Proof.
-    intros A P HP. unfold tau_invar in *.
-    pcofix CIH. pfold. 
-    constructor.
-    revert H t1 t2.
-    (*pcofix CIH.
-    split.
-    -*)
 
-  Admitted.
-*)
+(*Derives contradiction from evidence that a return tree is divergent*)
 Ltac inv_div_ret := match goal with [ H : divergenceF _ (RetF _) |- _  ] => inversion H end.
+
+(*Divergent trees never return a value*)
 Lemma div_ret_eutt : forall (E : Type -> Type) (A : Type) (t: itree E A) (a : A),
       divergence t -> ~(t ≈ ret a).
   Proof.
     intros. intros HContra. rewrite HContra in H. pinversion H.
   Qed.  
 
+(*Trees that return a value do not diverge*)
 Lemma ret_eutt_div : forall (E : Type -> Type) (A : Type) (t : itree E A) (a : A),
       t ≈ ret a -> ~ (divergence t).
   Proof.
     intros. intros HContra. rewrite H in HContra. pinversion HContra.
   Qed.
 
+(*spin is the only divergent itree with the Void event type,*)
 Lemma div_spin_eutt : forall (A : Type) (t : itree Void A), divergence t -> t ≈ spin.
 Proof.
   intros A. pcofix CIH. intros. pfold. red. cbn.
@@ -125,20 +97,26 @@ Proof.
   - destruct e.
 Qed.
 
+(*Formalized notion of specification monads and effect observations for pure, possibly divergent, computations *)
 Section PureITree.
   
   Definition PureITree A := itree Void A.
 
+  (*Morally, this is the type of pure itree specifcations. A sigma of this with a monotonicity requiremnet is used
+    in order to proved the ordered monad law*)
   Definition _PureITreeSpec A := forall (p : itree Void A -> Prop), (resp_eutt Void A p) -> Prop.
 
-  Definition _retpi A (a : A) : _PureITreeSpec A := fun p _ => p (ret a).
 
+
+  (*Monotonicity condition for specs on pure itrees*)
   Definition monotonici A (w : _PureITreeSpec A) :=
     forall (p p' : itree Void A -> Prop) (Hp : resp_eutt Void A p) (Hp' : resp_eutt Void A p'),
                                           (forall i', p i' -> p' i') -> w p Hp -> w p' Hp'. 
 
+  (*Sigm*)
   Definition PureITreeSpec A := {w : _PureITreeSpec A | monotonici A w}.
 
+  (*The set of predicates that accept divergent trees*)
   Definition _div_spec A : _PureITreeSpec A := fun p _ => p spin.
 
   Lemma div_spec_monot : forall A, monotonici A (_div_spec A).
@@ -147,13 +125,10 @@ Section PureITree.
     Qed.
 
   Definition div_spec A := exist _ (_div_spec A) (div_spec_monot A).
-    
 
-  Lemma retpi_monot : forall A (a : A), monotonici A (_retpi A a).
-  Proof.
-    unfold monotonici. intuition. unfold _retpi in *. auto.
-  Qed.
-
+  (*Assortment of definitions and lemmas defining an inductive definition of the return value of a tree and relating
+    it to tau_invar and divergence. I believe none of this code is particularly useful anymore*)
+  Section IsVal.
   Inductive is_val A (a : A) : itree Void A -> Prop :=
     | base :  is_val A a (ITreeDefinition.Ret a)
     | tau (t : itree Void A): is_val A a t -> is_val A a (Tau t) .
@@ -265,10 +240,20 @@ Section PureITree.
       - apply H. destruct Hcontra as [a Ha]. exists a. inv Ha. auto.
       - apply H. destruct Hcontra as [a Ha]. exists a. constructor. auto.
     Qed.
+  End IsVal.
+  (*End of deprecated section*)
+
+  (*Morally, this is the return function. This is paired with a proof that all such specs are monotonic*)
+  Definition _retpi A (a : A) : _PureITreeSpec A := fun p _ => p (ret a).
+
+  Lemma retpi_monot : forall A (a : A), monotonici A (_retpi A a).
+  Proof.
+    unfold monotonici. intuition. unfold _retpi in *. auto.
+  Qed.
 
   Lemma eutt_reta_or_div_aux : forall A (t : itree Void A), ~(exists a, ret a ≈ t) -> divergence t.
     Proof.
-      intro A. pcofix CIH. pfold. unfold divergence_.  intros. destruct (observe t) eqn : Heqt.
+      intro A. pcofix CIH. pfold. unfold divergence_. intros. destruct (observe t) eqn : Heqt.
       - exfalso. specialize (itree_eta t) as H. rewrite Heqt in H. apply H0.
          exists r0. rewrite H. reflexivity.
        - constructor. right. eapply CIH; eauto. intro. apply H0.
@@ -277,13 +262,14 @@ Section PureITree.
        - destruct e.
     Qed.
 
+  (*All itrees with Void event type either just return a value a, or they diverge (requires the law of the excluded middle to prove) *)
   Lemma eutt_reta_or_div : forall A (t : itree Void A), (exists a, ret a ≈ t) \/ (divergence t).
     Proof.
       intros A t.  specialize (classic (exists a, ret a ≈ t) ) as Hlem. destruct Hlem; auto.
       right. apply eutt_reta_or_div_aux. auto.
     Qed.
 
-
+  (*Proof that the predicate used in the bind function respects eutt*)
   Lemma bind_pred_resp_eutt : forall A B (f : A -> _PureITreeSpec B)
                                      (p : itree Void B -> Prop) (Hp : resp_eutt Void B p),
       resp_eutt Void A (fun (t : itree Void A) => (exists a, ret a ≈ t /\ f a p Hp) \/ 
@@ -308,21 +294,23 @@ Section PureITree.
     - rewrite <- Heutt in H. auto.
   Qed.    
   
-  (*intuitively, you have two choices, prove the tree evaluates to a and prove f a p,
+  (*the bind function for the PureITreeSpec monad
+    intuitively, you have two choices, prove the tree evaluates to a and prove f a p,
     or prove t is infinite and prove that the infinite predicate is in w*)
   Definition _bindpi A B (w : _PureITreeSpec A) (f : A -> _PureITreeSpec B) :=
     fun (p : itree Void B -> Prop) (Hp : resp_eutt Void B p) =>
       w (fun (t : itree Void A) => (exists a, ret a ≈ t /\ f a p Hp) \/ 
                                    (divergence t /\  p spin ))
   (bind_pred_resp_eutt A B f p Hp).
-(* replace   *)
 
+  (*Possible alternate bind*)
   Definition _bindpi' A B (w : _PureITreeSpec A) (f : A -> _PureITreeSpec B) :=
     fun (p : itree Void B -> Prop) (Hp : resp_eutt Void B p) =>
       w (fun (t : itree Void A) => (exists a, ret a ≈ t /\ f a p Hp) \/
                                    (divergence t /\ w divergence (divergence_resp_eutt A) /\ p spin) )
         (bind_pred_resp_eutt' A B f p Hp w).
- (*new div pre, (divergence t /\ w div _ /\ p spin)   *)
+ 
+
   Lemma bindpi_monot : forall A B (w : _PureITreeSpec A) (f : A -> _PureITreeSpec B),
       monotonici A w -> (forall a, monotonici B (f a)) -> monotonici B (_bindpi A B w f).
   Proof.
@@ -357,10 +345,11 @@ Section PureITree.
       eapply H0; eauto.
   Qed.
   
-
+  (*Definition of ret accounting for the proof of monotonicity*)
   Definition retpi A (a : A) : PureITreeSpec A :=
     exist _ (_retpi A a) (retpi_monot A a).
 
+  (*Definition of bind accounting for the proof of monotonicity*)
   Definition bindpi A B (w : PureITreeSpec A) (f : A -> PureITreeSpec B) :=
     let '(exist _ w' Hw') := w in
     let f' := fun a => proj1_sig (f a) in
@@ -372,9 +361,12 @@ Section PureITree.
     let f' := fun a => proj1_sig (f a) in
     let Hf' := fun a => proj2_sig (f a) in
     exist _ (_bindpi' A B w' f') (bindpi_monot' A B w' f' Hw' Hf').
+
+  (*Monad equivalence relation for PureITreeSpec monad *)
   Global Instance PureITreeSpecEq : EqM PureITreeSpec :=
     fun A w1 w2 => forall (p : itree Void A -> Prop) (Hp : resp_eutt Void A p), proj1_sig w1 p Hp <-> proj1_sig w2 p Hp.
 
+  
   Lemma ret_not_div : forall (A : Type) (E : Type -> Type) (a : A), ~ (@divergence E A (ret a)).
     Proof.
       intros. intro Hcontra. pinversion Hcontra.
@@ -394,6 +386,8 @@ Section PureITree.
       bind := bindpi
     }.
 
+
+  (*Monad law proofs*)
   Lemma retpi_bindpi : forall A B (f : A -> PureITreeSpec B) (a : A), 
       bind (ret a) f ≈ f a.
     Proof.
@@ -404,12 +398,11 @@ Section PureITree.
           apply inv_ret in Hvala0. subst. auto.
         + exfalso. destruct H. eapply ret_not_div. eauto.
       - simpl. destruct (f a) as [fa Hfa] eqn : Heq. simpl. intros.
-        left. exists a. split; auto.
+        left. exists a. split.
         + reflexivity.
         + rewrite Heq. auto.
     Qed.
 
-    
   Lemma bindpi_retpi : forall A (w : PureITreeSpec A), bind w (fun x => ret x) ≈ w.
   Proof.
     intros. destruct w as [ w Hw]. split.
@@ -425,8 +418,9 @@ Section PureITree.
       eapply Hw. 2: apply H. intros. unfold _retpi.
       specialize (eutt_reta_or_div A i') as Hor. destruct Hor.
       + destruct H1 as [a Ha]. left. exists a. split; auto. eapply Hp; eauto.
-      + right. split; auto. specialize (div_spin_eutt A i' H1) as H2. eapply Hp; eauto. symmetry. auto.
+      + right. split; auto. specialize (div_spin_eutt A i' H1) as H2. symmetry in H2. eapply Hp; eauto.
    Qed.
+
   Lemma bindpi_bindpi : forall (A B C : Type) (w : PureITreeSpec A) 
                                (f : A -> PureITreeSpec B) (g : B -> PureITreeSpec C),
       bind (bind w f) g ≈ bind w (fun a => bind (f a) g).
@@ -468,7 +462,7 @@ Section PureITree.
     destruct H2 as [a [Hreta Hf2a] ]. left. specialize (H0 a p Hp). exists a. auto.
   Qed.
 
-    
+  (*Definition of effect observation from pure itrees into pure itree specs *)
   Definition _obsip A (t : itree Void A) : _PureITreeSpec A := fun p _ => p t.
 
   Lemma obsip_monot : forall A (t : itree Void A), monotonici A (_obsip A t).
@@ -479,13 +473,7 @@ Section PureITree.
   Definition obsip A (t : itree Void A) : PureITreeSpec A :=
     exist _ (_obsip A t) (obsip_monot A t).
 
-(*
-  Instance ITreeVoidMonad : Monad (itree Void) :=
-    {
-      ret := ret;
-      bind := @bind;
-    }.
-*)
+  (*Proof that this effect observation is a valid monad morphism*)
   Lemma obsip_pres_ret : forall A (a : A), obsip A (ret a) ≈ ret a.
     Proof.
       intros. intros p Hp. cbn. unfold _retpi, _obsip. tauto.
@@ -601,7 +589,181 @@ Section StateITree.
   
   Definition StateITree A := itree (stateE S) A.
 
-  Definition _StateITreeSpec A := (itree Void (A * S) -> Prop) -> S -> Prop.
+  Definition _StateITreeSpec A := forall (p : itree Void (A * S) -> Prop), resp_eutt Void (A * S) p -> S -> Prop.
+
+  Definition monotonicsi A (w : _StateITreeSpec A) := forall (p p' : itree Void (A * S) -> Prop) 
+                                                             Hp Hp' s, (forall t, p t -> p' t) -> w p Hp s -> w p' Hp' s.
+
+  Definition StateITreeSpec A := {w : _StateITreeSpec A | monotonicsi A w}.
+
+  Definition _retsi A (a : A) : _StateITreeSpec A := fun p _ s => p (ret (a,s)).
+
+  Lemma monot_retsi : forall A (a : A), monotonicsi A (_retsi A a).
+    Proof.
+      intros. unfold _retsi. intros p p' _ _ s. intros. apply H. auto.
+    Qed.
+
+  Definition retsi A (a : A) : StateITreeSpec A := exist _ (_retsi A a) (monot_retsi A a).
+
+  Lemma bindsi_pred_eutt : forall A B (w : _StateITreeSpec A) (f : A -> _StateITreeSpec B) 
+                                  (p : itree Void (B * S) -> Prop) (Hp : resp_eutt Void (B * S) p) (s : S), 
+         resp_eutt Void (A * S) (fun t => (exists a s', ret (a,s') ≈ t /\ f a p Hp s') \/ divergence t /\ p spin).
+  Proof.
+    intros. intros t1 t2 Heutt. split; intros.
+    - destruct H.
+      + destruct H as [a [s' [Hretas Hfa ] ] ]. left. exists a. exists s'. split; auto.
+        rewrite Hretas. auto.
+      + right. rewrite <- Heutt. auto.
+    - destruct H.
+      + destruct H as [a [s' [Hretas Hfa ] ] ]. left. exists a. exists s'. split; auto.
+        rewrite Heutt. auto.
+      + right. rewrite <- Heutt in H. auto.
+   Qed.
+
+  Definition _bindsi A B (w : _StateITreeSpec A) (f : A -> _StateITreeSpec B) :=
+    fun (p : itree Void (B * S) -> Prop) (Hp : resp_eutt Void (B * S) p) (s : S) =>
+      w (fun (t : itree Void (A * S) )=> (exists a s', ret (a,s') ≈ t /\ f a p Hp s' )  \/ 
+                                         (divergence t /\ p spin) )  
+        (bindsi_pred_eutt A B w f p Hp s) s.
+
+  Lemma monot_bindsi : forall A B (w : _StateITreeSpec A) (f : A -> _StateITreeSpec B), monotonicsi A w ->
+      (forall a, monotonicsi B (f a)) -> monotonicsi B (_bindsi A B w f).
+  Proof.
+    unfold monotonicsi. intros. unfold _bindsi in *.
+    set (fun (t : itree Void (A * S)) p0 Hp0 => (exists a s', ret (a,s') ≈ t /\ f a p0 Hp0 s') \/ (divergence t /\ p0 spin)) as fp.
+    enough (forall t, fp t p Hp -> fp t p' Hp').
+    - eapply H with (p := fun t => fp t p Hp); eauto.
+    - unfold fp. intros. destruct H3.
+      + left. destruct H3 as [a [s' [Hretas' Hfa] ] ].
+        exists a. exists s'. split; auto. eapply H0; eauto.
+      + right. destruct H3. split; auto.
+  Qed.
+
+  Definition bindsi A B (w : StateITreeSpec A) (f : A -> StateITreeSpec B) : StateITreeSpec B :=
+             let '(exist _ w' Hw') := w in
+             let f' := fun a => proj1_sig (f a) in
+             let Hf' := fun a => proj2_sig (f a) in 
+             exist _ (_bindsi A B w' f') (monot_bindsi A B w' f' Hw' Hf').
+
+  Global Instance StateITreeSpecEq : EqM StateITreeSpec :=
+    fun A (w1 w2 : StateITreeSpec A) => forall p Hp s, proj1_sig w1 p Hp s <-> proj1_sig w2 p Hp s.
+
+  Global Instance StateITreeSpecMonad : Monad StateITreeSpec :=
+    {
+      ret := retsi;
+      bind := bindsi;
+    }.
+
+    (*Monad law proofs*)
+  Lemma retsi_bindsi : forall A B (f : A -> StateITreeSpec B) (a : A), 
+      bind (ret a) f ≈ f a.
+    Proof.
+      intros. split.
+      - cbn. unfold _bindsi, _retsi. intros. destruct H.
+        + destruct H as [a0 [s' [Haa0 Hfa0] ] ]. apply inv_ret in Haa0. injection Haa0 as H. subst. auto.
+        + destruct H. exfalso. eapply ret_not_div; eauto.
+      - cbn. unfold _bindsi, _retsi. intros. left. exists a. exists s.
+        split; auto. reflexivity.
+   Qed.
+
+  Lemma bindsi_retsi : forall A (w : StateITreeSpec A), bind w (fun x => ret x) ≈ w.
+  Proof.
+    intros. destruct w as [ w Hw]. split.
+    - cbn. unfold _bindsi, _retsi. intros. eapply Hw; try (apply H). intros.
+      destruct H0.
+      + destruct H0 as [ a [s' [Hretas' Has'] ] ]. symmetry in Hretas'. eapply Hp; eauto.
+      + destruct H0. apply div_spin_eutt in H0. eapply Hp; eauto.
+    - cbn. unfold _bindsi, _retsi. intros. eapply Hw; try (apply H). intros.
+      specialize (eutt_reta_or_div (A * S) t). intros. destruct H1.
+      + destruct H1 as [ [a s']  Hretas']. left. exists a. exists s'. split; auto.
+        eapply Hp; eauto.
+      + right. split; auto. eapply Hp; eauto. apply div_spin_eutt in H1. symmetry. auto.
+   Qed.
+
+  Lemma bindsi_bindsi : forall A B C (w : StateITreeSpec A) (f : A -> StateITreeSpec B) (g : B -> StateITreeSpec C), 
+      bind (bind w f) g ≈ bind w (fun a => bind (f a) g).
+  Proof.
+    intros. destruct w as [w Hw]. split; cbn.
+    - unfold _bindsi. intros. eapply Hw; try (apply H). intros. simpl in H0. clear H.
+      destruct H0.
+      + destruct H as [a [s' H ] ]. destruct H. destruct (f a) as [fa Hfa] eqn : Heq. simpl in *.
+        left. exists a. exists s'. split; auto.rewrite Heq. simpl. eapply Hfa; (try apply H0).
+        intros. destruct H1; auto.
+      + destruct H. destruct H0.
+        * destruct H0 as [b [s'' [Hretbs'' Hga] ] ]. exfalso.
+          specialize (spin_div Void (B* S) ) as H0. rewrite <- Hretbs'' in H0. pinversion H0.
+        * right. tauto.
+   - unfold _bindsi. intros. eapply Hw; try (apply H). simpl in *. intros. clear H. destruct H0.
+     + destruct H as [a [s' H] ]. destruct H. left. exists a. exists s'. split; auto.
+       destruct (f a) as [fa Hfa]. simpl in *. eapply Hfa; try apply H0. intros.
+       destruct H1; auto.
+     + destruct H. right. split; auto. right. split; auto. apply spin_div.
+  Qed.
+        
+  Global Instance StateITreeSpecMonadLaws : MonadLaws StateITreeSpec.
+  Proof.
+    constructor.
+    - apply retsi_bindsi.
+    - apply bindsi_retsi.
+    - apply bindsi_bindsi.
+  Qed.
+
+  Global Instance StateITreeSpecOrderM : OrderM StateITreeSpec :=
+    fun A (w1 w2 : StateITreeSpec A) => forall p Hp s, proj1_sig w2 p Hp s -> proj1_sig w1 p Hp s.
+
+  Global Instance StateITreeSpecOrderLaws : OrderedMonad StateITreeSpec.
+  Proof.
+    intros A B w1 w2 f1 f2. intros. destruct w1 as [w1 Hw1]. destruct w2 as [w2 Hw2]. cbn in *.
+    intros p Hp s. cbn. unfold _bindsi. intros. apply H. simpl. eapply Hw2; try apply H1.
+    intros. destruct H2; auto.
+    destruct H2 as [a [s' [Hretas' Hf2a] ] ]. left. exists a. exists s'. split; auto.
+    apply H0. auto.
+  Qed.
+
+  Definition _obssi A (m : S -> itree Void (A * S)) : _StateITreeSpec A :=
+    fun post Hp s => post (m s).
+
+  Lemma monot_obssi : forall A (m : S -> itree Void (A * S)), monotonicsi A (_obssi A m).
+  Proof.
+    unfold monotonicsi. intros. apply H. auto.
+  Qed.
+
+  Definition obssi A (m : S -> itree Void (A * S) ) : StateITreeSpec A :=
+    exist _ (_obssi A m) (monot_obssi A m).
+
+  Definition ret_stateitree A (a : A) : (S -> itree Void (A * S) ):= fun s => ret (a,s).
+
+  Definition bind_stateitree A B (m : S -> itree Void (A * S) ) (f : A -> (S -> itree Void (B * S))) : S -> (itree Void (B * S)) :=
+    fun s => let t := m s in bind t (fun '(a,s') => f a s' ) .
+
+  Global Instance StateTransformITreeMonad : Monad (fun A => S -> itree Void (A * S)) :=
+    {
+      ret := ret_stateitree;
+      bind := bind_stateitree;
+    }.
+
+  Lemma obssi_pres_ret : forall A (a : A), obssi A (ret a) ≈ ret a.
+  Proof.
+    intros. cbn. intros p Hp s. split; intros; apply H.
+  Qed.
+
+  Lemma obssi_pres_bind : forall A B (m : S -> itree Void (A * S) ) (f : A -> S -> itree Void (B * S)),
+      obssi B (bind m f) ≈ bind (obssi A m) (fun a => obssi B (f a) ).
+  Proof.
+    intros. cbn. intros p Hp s. split; intros.
+    - simpl in *. unfold bind_stateitree in H. unfold _obssi in H.
+      unfold _bindsi. unfold _obssi.
+      specialize (eutt_reta_or_div _ (m s) ) as Hor. destruct Hor.
+      * left. destruct H0 as [ [a s' ] Has']. exists a. exists s'. split; auto.
+        eapply Hp; eauto. rewrite <- Has'. simpl. symmetry. specialize (bind_ret (a,s') (fun '(a0,s0) => f a0 s0) ) as H1.
+        simpl in H1. rewrite H1. reflexivity.
+      * right. split; auto. apply div_spin_eutt in H0. eapply Hp; eauto. rewrite H0. apply spin_bind.
+    - simpl in *. unfold bind_stateitree. unfold _bindsi, _obssi in *. destruct H.
+      + destruct H as [a [s' [Hretas' Hpfa] ] ]. eapply Hp; eauto. rewrite <- Hretas'.
+        specialize (bind_ret (a,s') (fun '(a0,s0) => f a0 s0 ) ) as H1. simpl in H1. rewrite H1. reflexivity.
+      + destruct H. eapply Hp; eauto. apply div_spin_eutt in H. rewrite H. symmetry. apply spin_bind.
+  Qed.
+   
 End StateITree.
 (*
   Definition _interpStateSpec : (stateE S) ~> (_StateSpec S) :=
